Source/CS.v
@@ -40,6 +40,13 @@ Inductive cont : Type :=
 | Kassign2 (v: value) (k: cont)
 | Kcall (C: Component.id) (P: Procedure.id) (k: cont).
 
+Lemma continuation_absurd : forall k e1 e2,
+    Kseq (E_seq e1 e2) k <> k.
+Proof.
+  elim => // e k IHk e1 e2 Hkseq.
+  inversion Hkseq as [[He Hind]]. by apply IHk in Hind.
+Qed.
+
 Module CS.
 
 CoInductive frame : Type := Frame {
@@ -693,6 +700,376 @@ Section Semantics.
 
 
   Admitted.
+
+  Lemma all_expressions_evaluate (* cs_i t_i *) C s mem k e arg :
+
+    (* Is this the right way to state that e is well typed ? (you can get from
+       the initial state of the program to the expr e, and p is well typed so is
+       e) *)
+    (* initial_state p cs_i -> *)
+    (* Star sem cs_i t_i [State C, s, mem, k, e, arg] -> *)
+
+    (* Or maybe is there a more usable way to say that e is well_typed ? *)
+    well_formed_expr p C e ->
+
+    exists mem' t v,
+      Star sem
+           [State C, s, mem,  k, e,       arg] t
+           [State C, s, mem', k, E_val v, arg].
+  Proof.
+    (* intro Hinitial. *)
+    move: (* t_i *) C s mem k arg.
+    induction e as [ v | b | |
+                     bin e1 IHe1 e2 IHe2 |
+                     e1 IHe1 e2 IHe2 |
+                     e__if IHe__if e__then IHe__then e__else IHe__else |
+                     e__alloc IHe__alloc |
+                     e__deref IHe__deref |
+                     e__assign IHe__assign e__val IHe__val |
+                     Cid Pid P__expr IHP__expr |
+                     Cid | ]=> C s mem k arg Hwf_e.
+      - (* E_val *)
+        exists mem, E0, v ; by apply star_refl.
+      - (* E_arg *)
+        exists mem, E0 ; eexists ; eapply star_one.
+        (* eapply KS_Arg *)
+        destruct arg ; simpl ; rewrite -eval_kstep_correct ; simpl ;
+          first done ; exfalso ;
+        (* simpl in Hstep. rewrite <- eval_kstep_correct in Hstep. *)
+        (* inversion valid_program as [? ? ? wf_proc ? ? ?]. *)
+        (* inversion complete_program. simpl in Hstar. *)
+        (* (* simpl in Hstar. *) *)
+        (* (* generalize dependent e3 ; generalize dependent e2. *) *)
+        (* (* unfold prepare_global_env in G. simpl. unfold G. intro z. *) *)
+        (* (* simpl. *) *)
+        (* admit. *)
+        (** Should be stuck (cannot have Ptr or Undef as arg in a wf_prog and more precisely in a wf_expr), how to show it ? *)
+            admit.
+      - (* E_local *)
+        exists mem, E0 ;
+          by destruct b ; eexists ; eapply star_one ; constructor.
+      - (* E_binop *)
+        destruct Hwf_e as [Hvalid_calls Hval_int ]. simpl in Hvalid_calls, Hval_int.
+        move:Hval_int => /andP[Hval_int_e1 Hval_int_e2].
+        have Hvalid_equiv: valid_calls (prog_procedures p) (prog_interface p) C
+                          (called_procedures e1 :|: called_procedures e2) ->
+              valid_calls (prog_procedures p) (prog_interface p) C
+                          (called_procedures e1) /\
+              valid_calls (prog_procedures p) (prog_interface p) C
+                          (called_procedures e2) by admit.
+        apply Hvalid_equiv in Hvalid_calls.
+        move: Hvalid_calls {Hvalid_equiv} => [Hvalid_calls_e1 Hvalid_calls_e2].
+        have Hwf_e1: well_formed_expr p C e1 by split.
+        have Hwf_e2: well_formed_expr p C e2 by split.
+        specialize (IHe1 C s mem (Kbinop1 bin e2 k) arg Hwf_e1).
+        (* inversion Hstar_initial ; subst. inversion Hinitial. unfold initial_machine_state in H0. *)
+        destruct IHe1 as [mem1 [?t [v1 star_e1]]].
+        specialize (IHe2 C s mem1  (Kbinop2 bin v1 k) arg Hwf_e2).
+        destruct IHe2 as [?mem [t2 [v2 star_e2]]].
+        do 3 eexists.
+        eapply star_step with (t1:=E0) ; last by rewrite E0_left.
+        apply KS_Binop1. (* specialize IHe1_1 with (c:= Kbinop1 b e1_2 c) (mem:= mem). *)
+        (* destruct IHe1_1 as [mem1 [?t [v1 star_e1_1]]]. *)
+        eapply star_trans ; first by apply star_e1.
+        eapply star_step with (t1:=E0) ; last by rewrite E0_left.
+        apply KS_Binop2. (* specialize IHe1_2 with (c:= Kbinop2 b v1 c) (mem:= mem1). *)
+        (* destruct IHe1_2 as [?mem [t2 [v2 star_e1_2]]]. *)
+        eapply star_trans with (t1:=t2) (t2:=E0) ;
+          last rewrite E0_right ;
+          first by apply star_e2.
+        apply star_one. by apply KS_BinopEval. done. done.
+      - (* E_seq *)
+
+        admit.
+      - (* E_if *)
+        admit.
+      - (* E_alloc *)
+        admit.
+      - (* E_deref *)
+        admit.
+      - (* E_assign *)
+        admit.
+      - (* E_call *)
+        admit.
+      - (* E_component_buf *)
+  Admitted.
+
+  (*
+| KS_Seq1 :  forall C s mem k e1 e2 arg,
+    kstep G [State C, s, mem, k, E_seq e1 e2, arg] E0
+            [State C, s, mem, Kseq e2 k, e1, arg]
+| KS_Seq2 : forall C s mem k v e2 arg,
+    kstep G [State C, s, mem, Kseq e2 k, E_val v, arg] E0
+            [State C, s, mem, k, e2, arg]
+   *)
+
+(** we should have something like :
+(Left side)
+ Plus sem [State C, s, mem0, k, E_seq (E_seq e1 e2) e3, arg] evs
+          [State C, s, mem__final, k, e3, arg]
+          ≜
+ (KS_Seq1)
+ Step sem [State C, s, mem0, k, E_seq (E_seq e1 e2) e3, arg] E0
+          [State C, s, mem0, Kseq e3 k, E_seq e1 e2, arg]
+ **
+ (KS_Seq1)
+ Step sem [State C, s, mem0, Kseq e3 k, E_seq e1 e2, arg] E0
+          [State C, s, mem0, Kseq e2 (Kseq e3 k), e1, arg]
+ **
+ (This is the part where case analysis/induction on e1 happens )
+ Star sem [State C, s, mem0, Kseq e2 (Kseq e3 k), e1, arg] t1
+          [State C, s, mem1, Kseq e2 (Kseq e3 k), E_val v, arg]
+ (mem1 may be different from mem0, and t1 may be non empty)
+ **
+ (KS_Seq2)
+ Step sem [State C, s, mem1, Kseq e2 (Kseq e3 k), E_val v, arg] E0
+          [State C, s, mem1, Kseq e3 k, e2, arg]
+ (case analysis/induction on e2)
+ Star sem [State C, s, mem1, Kseq e3 k, e2, arg] t2
+          [State C, s, mem__final, Kseq e3 k, E_val v, arg]
+ **
+ (KS_Seq2)
+ Step sem [State C, s, mem__final, Kseq e3 k, E_val v, arg] E0
+          [State C, s, mem__final, k, e3, arg]
+
+And (Right side)
+ Plus sem [State C, s, mem0, k, E_seq e1 (E_seq e2 e3), arg] evs
+          [State C, s, mem__final, k, e3, arg]
+          ≜
+ (KS_Seq1)
+ Step sem [State C, s, mem0, k, E_seq e1 (E_seq e2 e3), arg] E0
+          [State C, s, mem0, Kseq (E_seq e2 e3) k, e1, arg]
+ **
+ (case analysis/induction on e1)
+ Star sem [State C, s, mem0, Kseq (E_seq e2 e3) k, e1, arg] t1
+          [State C, s, mem1, Kseq (E_seq e2 e3) k, E_val v, arg]
+ **
+ (KS_Seq2)
+ Step sem [State C, s, mem1, Kseq (E_seq e2 e3) k, E_val v, arg] E0
+          [State C, s, mem1, k, E_seq e2 e3, arg]
+ **
+ (KS_Seq1)
+ Step sem [State C, s, mem1, k, E_seq e2 e3, arg] E0
+          [State C, s, mem1, Kseq e3 k, e2, arg]
+ **
+ (case analysis/induction on e2)
+ Star sem [State C, s, mem1, Kseq e3 k, e2, arg] t2
+          [State C, s, mem2, Kseq e3 k, E_val v, arg]
+ **
+ (KS_Seq2)
+ Step sem [State C, s, mem2, Kseq e3 k, E_val v, arg] E0
+          [State C, s, mem2, k, e3, arg]
+
+We can even draw the finish line right before the case/ind on e2 since it's exactly the same from here *)
+  (* Conjecture seq_associative : associative E_seq. *)
+  (* Ltac inversion_star_and_subst := *)
+  (*   match goal with *)
+  (*   | H: Kseq (E_seq _ _ ) ?k = ?k |- _ => *)
+  (*     inversion_clear H as [H H' H'' [H''' Hcontra H'''1]|] ; subst *)
+  (*   | _  => idtac *)
+  (*   end. *)
+
+  Lemma seq_assoc_in_CS_aux_left_seq C s mem mem' k e1 e2 e3 arg evs:
+      Plus sem
+           [State C, s, mem, k, E_seq (E_seq e1 e2) e3, arg] evs
+           (* [State C, s, mem', Kseq e3 k, e2, arg] *)
+           (* Or *)
+           [State C, s, mem', k, e3, arg]
+      -> Plus sem
+           [State C, s, mem, k, E_seq e1 (E_seq e2 e3), arg] evs
+           [State C, s, mem', Kseq e3 k, e2, arg].
+  Proof.
+    intro H.
+    apply plus_trans with (t1:=E0)
+                          (t2:=evs)
+                          (s2:= [State C, s, mem, Kseq (E_seq e2 e3) k, e1, arg]);
+      last by rewrite E0_left.
+    apply plus_one, KS_Seq1.
+    have:  exists mem' t v,
+        Star sem
+             [State C, s, mem, Kseq (E_seq e2 e3) k, e1, arg] t
+             [State C, s, mem', Kseq (E_seq e2 e3) k, E_val v, arg]
+    (* \/ *)
+        (* Plus sem *)
+        (*      [State C, s, mem, Kseq (E_seq e2 e3) k, e1, arg] t *)
+        (*      [State C, s, mem', Kseq (E_seq e2 e3) k, E_val v, arg] *).
+    {
+      apply all_expressions_evaluate. admit.
+      (* inversion_clear H as [? ? ? ? ? ? Hstep Hstar (* ... *)] ; subst ; *)
+      (*   inversion Hstep ; subst. *)
+      (* inversion Hstar as [state Hstate Htrace [Hmem Hcontra Hexp]| state1 trace1 state2 trace2 state3 trace3 Hstep' Hstar' Htrace] ; subst ; *)
+      (*   (* inversion_star_and_subst *) *)
+      (*   (* [>by apply continuation_absurd in Hcontra| ..] *) *)
+      (*   (** Not strong enough since we know that all the first goals generated by *)
+      (*    inversion Hstar must be solved by this, but the 'subst' in between cannot *)
+      (*    allow us to use 'first' *) *)
+      (*   (* try by apply continuation_absurd in Hcontra. *) *)
+      (*   match goal with *)
+      (*   | H: Kseq (E_seq _ _ ) ?k = ?k |- _ => *)
+      (*       by apply continuation_absurd in H ; idtac "boup" *)
+      (*   | _  => idtac *)
+      (*   end. *)
+      (* (* move: Hstar Hstep Hstep' Hstar'. *) *)
+      (* generalize (Kseq (E_seq e2 e3) k). *)
+      (* clear Hstar Hstep Hstar' Hstep'. generalize dependent mem. *)
+      (* (* generalize dependent e3 ; generalize dependent e2. generalize dependent k. *) *)
+      (* induction e1 => mem c (* => k e2 e3 *) (* H Hstar Hstep *) *)
+      (* (* ; exists mem, E0 *) (* . eexists *) *)
+      (* (*       inversion Hstar as [H0 H' H'' [H''' Hcontra H'''1]|] ; subst ; *)
+      (*   (* inversion_star_and_subst *) *)
+      (*   (* [>by apply continuation_absurd in Hcontra| ..] *) *)
+      (*   (** Not strong enough since we know that all the first goals generated by *)
+      (*    inversion Hstar must be solved by this, but the 'subst' in between cannot *)
+      (*    allow us to use 'first' *) *)
+      (*   (* try by apply continuation_absurd in Hcontra. *) *)
+      (*   match goal with *)
+      (*   | H: Kseq (E_seq _ _ ) ?k = ?k |- _ => *)
+      (*       by apply continuation_absurd in H *)
+      (*   | _  => idtac *)
+      (*   end. *) *)
+      (* . *)
+      (* - (* E_val *) *)
+      (*   exists mem, E0, v ; by apply star_refl. *)
+      (* - (* E_arg *) *)
+      (*   exists mem, E0 ; eexists ; eapply star_one. *)
+      (*   (* eapply KS_Arg *) *)
+      (*   destruct arg ; simpl ; rewrite -eval_kstep_correct ; simpl ; *)
+      (*     first done ; exfalso ; *)
+      (*   (* simpl in Hstep. rewrite <- eval_kstep_correct in Hstep. *) *)
+      (*   (* inversion valid_program as [? ? ? wf_proc ? ? ?]. *) *)
+      (*   (* inversion complete_program. simpl in Hstar. *) *)
+      (*   (* (* simpl in Hstar. *) *) *)
+      (*   (* (* generalize dependent e3 ; generalize dependent e2. *) *) *)
+      (*   (* (* unfold prepare_global_env in G. simpl. unfold G. intro z. *) *) *)
+      (*   (* (* simpl. *) *) *)
+      (*   (* admit. *) *)
+      (*   (** Should be stuck (cannot have Ptr or Undef as arg in a wf_prog and more precisely in a wf_expr), how to show it ? *) *)
+      (*       admit. *)
+      (* - (* E_local *) *)
+      (*   exists mem, E0 ; *)
+      (*     by destruct b ; eexists ; eapply star_one ; constructor. *)
+      (* - (* E_binop *) *)
+      (*   specialize IHe1_1 with (c:= Kbinop1 b e1_2 c) (mem:= mem). *)
+      (*   destruct IHe1_1 as [mem1 [?t [v1 star_e1_1]]]. *)
+      (*   specialize IHe1_2 with (c:= Kbinop2 b v1 c) (mem:= mem1). *)
+      (*   destruct IHe1_2 as [?mem [t2 [v2 star_e1_2]]]. *)
+      (*   do 3 eexists. *)
+      (*   eapply star_step with (t1:=E0) ; last by rewrite E0_left. *)
+      (*   apply KS_Binop1. (* specialize IHe1_1 with (c:= Kbinop1 b e1_2 c) (mem:= mem). *) *)
+      (*   (* destruct IHe1_1 as [mem1 [?t [v1 star_e1_1]]]. *) *)
+      (*   eapply star_trans ; first by apply star_e1_1. *)
+      (*   eapply star_step with (t1:=E0) ; last by rewrite E0_left. *)
+      (*   apply KS_Binop2. (* specialize IHe1_2 with (c:= Kbinop2 b v1 c) (mem:= mem1). *) *)
+      (*   (* destruct IHe1_2 as [?mem [t2 [v2 star_e1_2]]]. *) *)
+      (*   eapply star_trans with (t1:=t2) (t2:=E0) ; *)
+      (*     last rewrite E0_right ; *)
+      (*     first by apply star_e1_2. *)
+      (*   apply star_one. by apply KS_BinopEval. done. done. *)
+
+    }
+        (* intro. destruct x. destruct H ; destruct H. *)
+    intros [mem1 [t1 [v1 Hstar]]].
+    inversion H as [? ? ? ? ? ? Hstep Hstar' (* ... *)] ; subst.
+    inversion Hstep ; subst.
+    (* inversion Hstar' as [|] ; subst. *)
+    (*   eapply star_plus_trans with (t1:=t1) *)
+    (*                               (t2:=E0) ; *)
+    (*     last (rewrite E0_right) ; *)
+    (*     first (by apply Hstar) ; clear Hstar. *)
+    (*   apply plus_trans with (t1:=E0) *)
+    (*                         (t2:=E0) *)
+    (*                         (s2:= [State C, s, mem', k, E_seq e2 e3, arg]); *)
+    (*     last by rewrite E0_left. *)
+    (*   apply plus_one, KS_Seq2. *)
+    (*   apply plus_one, KS_Seq1. *)
+  Admitted.
+
+  Lemma seq_assoc_in_CS_aux_right_seq C s mem mem' k e1 e2 e3 arg evs:
+      Plus sem
+           [State C, s, mem, k, E_seq e1 (E_seq e2 e3), arg] evs
+           (* [State C, s, mem', Kseq e3 k, e2, arg] *)
+           (* Or *)
+           [State C, s, mem', k, e3, arg]
+      -> Plus sem
+           [State C, s, mem, k, E_seq (E_seq e1 e2) e3, arg] evs
+           [State C, s, mem', Kseq e3 k, e2, arg].
+  Proof.
+  Admitted.
+
+  (* Not well stated at all, not true in general *)
+  Lemma seq_assoc_in_CS_aux_common:
+    forall C s mem mem' k e1 e2 e3 arg evs,
+      Plus sem
+           (* direction doesn't really matter at this point I guess *)
+           [State C, s, mem, k, E_seq (E_seq e1 e2) e3, arg] evs
+           [State C, s, mem', k, e3, arg] ->
+      Plus sem
+           [State C, s, mem, Kseq e3 k, e2, arg] evs
+           [State C, s, mem', k, e3, arg].
+  Proof.
+    intros.
+    have: exists v,
+        Star sem
+             [State C, s, mem, Kseq e3 k, e2, arg] evs
+             [State C, s, mem', Kseq e3 k, E_val v, arg].
+    induction e2 ; admit.
+    intros [v Hstar].
+    apply plus_right with (s2:=[State C, s, mem', Kseq e3 k, E_val v, arg])
+                           (t1:=evs)
+                           (t2:=E0) ;
+      last (by rewrite E0_right) ;
+      first (by apply Hstar) ; clear Hstar.
+    apply KS_Seq2.
+    Admitted.
+
+  Lemma seq_assoc_in_CS:
+  forall C s mem mem' k e1 e2 e3 arg evs,
+    (* If we can go from e1 to e3 ("legal" expressions) *)
+    (* Star *) Plus sem [State C, s, mem, k, E_seq (E_seq e1 e2) e3, arg] evs
+             [State C, s, mem', k, e3, arg] <->
+            (* then the sequencing doesn't matter, we have ((e1;e2); e3) <-> (e1;(e2;e3)) *)
+    (* Star *) Plus sem [State C, s, mem, k, E_seq e1 (E_seq e2 e3), arg] evs
+                    [State C, s, mem', k, e3, arg].
+
+    (* step kstep (prepare_global_env p) [State C, s, mem, k, E_seq (E_seq e1 e2) e3, arg] evs *)
+    (*      [State C, s, mem', k, e3, arg] <-> *)
+    (* step kstep (prepare_global_env p) [State C, s, mem, k, E_seq e1 (E_seq e2 e3), arg] evs *)
+    (*      [State C, s, mem', k, e3, arg]. *)
+
+  (*   (* NB : no need to have different `s` or `arg` since we sequence expressions in the same stack frame (if we make a function call, we should return from it before ending the sequence) *) *)
+Proof.
+  split ; intro Dir1.
+  (* - (* -> *) *)
+  (*   eapply plus_trans. *)
+  (*   eapply plus_trans in Dir1. *)
+  (*   eapply plus_trans ; [|eapply seq_assoc_in_CS_aux_common |]. *)
+  (*    apply seq_trans_in_CS_aux_left_seq. *)
+  (*   eapply (plus_trans seq_trans_in_CS_aux_left_seq seq_trans_in_CS_aux_common). *)
+  (* - (* <- *) *)
+  (*   inversion Dir1 as [? ? ? ? ? ? Hstep Hstar (* ... *)] ; subst. *)
+  (*   inversion Hstep ; subst. *)
+  (*   eapply plus_trans. repeat econstructor. 2: by rewrite !E0_left. *)
+  (*   eapply plus_trans. repeat econstructor. 2: by rewrite !E0_left. *)
+  (*   induction e1. *)
+  (*   + eapply plus_trans. *)
+  (*   (* have: Kseq e2 (Kseq e3 k) = Kseq (E_seq e2 e3) k. *) *)
+  (*   (* induction e1 => //. *) *)
+  (*   (* eapply plus_left'. *) *)
+  (*   apply star_inv in Hstar ; destruct Hstar as [[HcontraState ?] | Hstar] ; subst. *)
+  (*   + inversion HcontraState ; subst. *)
+  (*   (* inversion Hstar ; subst. *) *)
+  (*   + (* Dead-end, cannot have star_refl *) *)
+  (*     admit. *)
+  (*   + *)
+  (*   (* econstructor. constructor. econstructor. constructor. econstructor. *) *)
+  (*   repeat econstructor ; last rewrite !E0_left E0_right. *)
+  (*   (* inversion Hstep ; subst. *) *)
+  (*   induction e1 => //=. *)
+  (*   +  apply KS_Seq2. *)
+
+  (*   ; simpl in Dir1, Hstep, Hstar. *)
+  (* econstructor. *)
+Admitted.
 
 End Semantics.
 
